Simplify value optimization logic

theories/ValueOpts/ValueOpts.v
@@ -9,55 +9,53 @@ Set Implicit Arguments.
 Unset Printing Records.
 Print Coercions.
 
-Inductive eqn_sound : list params -> list (set var) -> list eqns  (*params*set var*eqns*)
+Inductive eqn_sound : list params -> list eqns  (*params*set var*eqns*)
                       -> stmt -> stmt
                       -> eqns
                       -> ann (set var * set var)
                       -> Prop :=
-| EqnLet x ZL Δ Γ  s s' e Gamma e' G G' ang
-  : eqn_sound ZL Δ Γ s s' {EqnEq (Var x) e ; Gamma } ang
-    (* make sure the rest conforms to the new assignment *)
+| EqnLet x ZL Δ s s' e Gamma e' G G' ang
+  : eqn_sound ZL Δ s s' {EqnEq (Var x) e ; Gamma } ang
     -> entails Gamma {EqnApx e e'}
-    -> eqn_sound ZL Δ Γ (stmtLet x (Operation e) s) (stmtLet x (Operation e') s') Gamma
+    -> eqn_sound ZL Δ (stmtLet x (Operation e) s) (stmtLet x (Operation e') s') Gamma
                 (ann1 (G,G') ang)
-| EqnIf ZL Δ Γ e e' s s' t t' Gamma G G' ang1 ang2
-  : eqn_sound ZL Δ Γ s s' {EqnEq (UnOp UnOpToBool e) (Con val_true); Gamma} ang1
-  -> eqn_sound ZL Δ Γ t t' {EqnEq (UnOp UnOpToBool e) (Con val_false); Gamma} ang2
+| EqnIf ZL Δ e e' s s' t t' Gamma G G' ang1 ang2
+  : eqn_sound ZL Δ s s' {EqnEq (UnOp UnOpToBool e) (Con val_true); Gamma} ang1
+  -> eqn_sound ZL Δ t t' {EqnEq (UnOp UnOpToBool e) (Con val_false); Gamma} ang2
   -> entails Gamma {(EqnApx e e')}
-  -> eqn_sound ZL Δ Γ (stmtIf e s t) (stmtIf e' s' t') Gamma
+  -> eqn_sound ZL Δ (stmtIf e s t) (stmtIf e' s' t') Gamma
               (ann2 (G,G') ang1 ang2)
-| EqnApp (l:lab) Y Y' ZL Δ Γ Gamma Z Γf Gf G G'
-  : get ZL  l Z -> get Δ l Gf -> get Γ l Γf
+| EqnApp (l:lab) Y Y' ZL Δ Gamma Z Γf G G'
+  : get ZL  l Z -> get Δ l Γf
     -> length Y = length Y'
     -> entails (of_list ((fun y => EqnEq y y) ⊝ Y') ∪ Gamma) (subst_eqns (sid [Z <-- Y']) Γf)
     -> entails Gamma (list_EqnApx Y Y')
-    -> eqn_sound ZL Δ Γ (stmtApp l Y) (stmtApp l Y') Gamma (ann0 (G,G'))
-| EqnReturn ZL Δ Γ e e' Gamma G G'
+    -> eqn_sound ZL Δ (stmtApp l Y) (stmtApp l Y') Gamma (ann0 (G,G'))
+| EqnReturn ZL Δ e e' Gamma G G'
   : entails Gamma {(EqnApx e e')}
-    -> eqn_sound ZL Δ Γ (stmtReturn e) (stmtReturn e') Gamma (ann0 (G,G'))
-| EqnExtern x f ZL Δ Γ s s' Y Y' Gamma G G' ang
-  : eqn_sound ZL Δ Γ s s' {EqnEq (Var x) (Var x) ; Gamma} ang
+    -> eqn_sound ZL Δ (stmtReturn e) (stmtReturn e') Gamma (ann0 (G,G'))
+| EqnExtern x f ZL Δ s s' Y Y' Gamma G G' ang
+  : eqn_sound ZL Δ s s' {EqnEq (Var x) (Var x) ; Gamma} ang
     -> entails Gamma (list_EqnApx Y Y')
     -> list_union (List.map Op.freeVars Y') ⊆ G
     -> length Y = length Y'
-    -> eqn_sound ZL Δ Γ (stmtLet x (Call f Y) s) (stmtLet x (Call f Y') s') Gamma
+    -> eqn_sound ZL Δ (stmtLet x (Call f Y) s) (stmtLet x (Call f Y') s') Gamma
                 (ann1 (G,G') ang)
-| EqnFun ZL Δ Γ ΓF F F' t t'  Gamma G G' angs angb
+| EqnFun ZL Δ ΓF F F' t t' Gamma G G' angs angb
          (Len1:length(ΓF) = length F)
          (Len2: length F = length F')
          (ParamEq:forall n Z s Z' s' , get F n (Z, s) -> get F' n (Z', s') -> Z = Z')
          (IndF:forall n Z s Z' s' EqS angn , get F n (Z, s) -> get F' n (Z', s')
                                         -> get ΓF n EqS -> get angs n angn
                                         -> eqn_sound (List.map fst F ++ ZL)
-                                                    ((List.map (fun _ => G) F) ++ Δ)
-                                                    (ΓF ++Γ)  s s' (EqS ∪ Gamma) angn)
-         (Indt:eqn_sound (List.map fst F ++ ZL) ((List.map (fun _ => G) F) ++ Δ) (ΓF ++Γ)  t t' Gamma angb)
+                                                    (ΓF ++ Δ) s s' (EqS ∪ Gamma) angn)
+         (Indt:eqn_sound (List.map fst F ++ ZL) (ΓF ++ Δ)  t t' Gamma angb)
          (EqnFVF: forall n EqS Zs, get F n Zs -> get ΓF n EqS -> eqns_freeVars EqS ⊆ G ∪ of_list (fst Zs))
-  : eqn_sound ZL Δ Γ (stmtFun F t) (stmtFun F' t') Gamma
+  : eqn_sound ZL Δ (stmtFun F t) (stmtFun F' t') Gamma
               (annF (G,G') angs angb)
-| EqnUnsat ZL Δ Γ s s' Gamma ang
+| EqnUnsat ZL Δ s s' Gamma ang
   : unsatisfiables Gamma
-    -> eqn_sound ZL Δ Γ s s' Gamma ang.
+    -> eqn_sound ZL Δ s s' Gamma ang.
 
 
 Lemma unsat_Equal Γ Γ'
@@ -70,35 +68,25 @@ Proof.
 Qed.
 
 Instance eqn_sound_Proper
-  : Proper (eq ==> list_eq Equal ==> eq ==> eq ==> eq ==> Equal ==> ann_R (@pe var _) ==> impl)
+  : Proper (eq ==> eq ==> eq ==> eq ==> Equal ==> ann_R (@pe var _) ==> impl)
            eqn_sound.
 Proof.
-  unfold Proper, respectful, impl; intros; subst. symmetry in H5.
-  general induction H6; only 1-6:(invt @ann_R; invt @pe).
-  - econstructor 1; eauto with cset; try rewrite <- H4; eauto.
-  - econstructor 2; eauto with cset; try rewrite <- H4; eauto.
-  - edestruct @list_eq_get; eauto; dcr.
-    econstructor 3; eauto with cset; try rewrite <- H6; eauto.
-  - econstructor 4; eauto with cset; try rewrite <- H4; eauto.
-  - econstructor 5; eauto with cset; try rewrite <- H4; eauto.
-    rewrite H11. eauto.
+  unfold Proper, respectful, impl; intros; subst. symmetry in H4.
+  general induction H5; only 1-6:(invt @ann_R; invt @pe).
+  - econstructor 1; eauto with cset; try rewrite <- H3; eauto.
+  - econstructor 2; eauto with cset; try rewrite <- H3; eauto.
+  - econstructor 3; eauto with cset; try rewrite <- H4; eauto.
+  - econstructor 4; eauto with cset; try rewrite <- H3; eauto.
+  - econstructor 5; eauto with cset; try rewrite <- H3; eauto.
+    rewrite H10. eauto.
   - econstructor 6; eauto with cset.
     + intros; inv_get.
       exploit H; eauto; try reflexivity.
-      eapply list_eq_app; eauto.
-      revert H8; clear.
-      induction F; simpl; eauto using @list_eq.
-      intros; econstructor; eauto. symmetry; eauto.
-      rewrite H4; eauto.
-    + eapply IHeqn_sound; eauto.
-      eapply list_eq_app; eauto.
-      revert H8; clear.
-      induction F; simpl; eauto using @list_eq.
-      intros; econstructor; eauto. symmetry; eauto.
+      rewrite H3; eauto.
     + intros; inv_get.
-      rewrite EqnFVF; eauto. rewrite H8. reflexivity.
+      rewrite EqnFVF; eauto. rewrite H7. reflexivity.
   - econstructor.
-    rewrite <- H4; eauto.
+    rewrite <- H3; eauto.
 Qed.
 
 
@@ -113,62 +101,6 @@ Ltac dowith c t :=
   match goal with
     | [ H : c _ _ _ _ |- _ ] => t H
   end.
-
-
-(*
-Lemma satisfies_update_dead_list E gamma Z vl
-: length Z = length vl
-  -> satisfies E gamma
-  -> freeVars gamma ∩ of_list Z [=] ∅
-  -> satisfies (E[Z <-- vl]) gamma.
-Proof.
-  intros. destruct gamma; simpl in * |- *.
-  - inv H0. symmetry in H3. symmetry in H2.
-    erewrite exp_eval_agree; try eapply H2.
-    symmetry.
-    erewrite exp_eval_agree; try eapply H3.
-    econstructor; reflexivity.
-    erewrite <- minus_inane_set. symmetry.
-    eapply update_with_list_agree_minus; eauto.
-    cset_tac; intuition. eapply (H1 a); cset_tac; intuition.
-    erewrite <- minus_inane_set. symmetry.
-    eapply update_with_list_agree_minus; eauto.
-    cset_tac; intuition. eapply (H1 a); cset_tac; intuition.
-  - inv H0.
-    + symmetry in H3.
-      erewrite exp_eval_agree; try eapply H3. econstructor.
-      erewrite <- minus_inane_set. symmetry.
-      eapply update_with_list_agree_minus; eauto.
-      cset_tac; intuition. eapply (H1 a); cset_tac; intuition.
-    + symmetry in H3. symmetry in H2.
-      erewrite exp_eval_agree; try eapply H2.
-      erewrite exp_eval_agree; try eapply H3.
-      econstructor; reflexivity.
-      erewrite <- minus_inane_set. symmetry.
-      eapply update_with_list_agree_minus; eauto.
-      cset_tac; intuition. eapply (H1 a); cset_tac; intuition.
-      erewrite <- minus_inane_set. symmetry.
-      eapply update_with_list_agree_minus; eauto.
-      cset_tac; intuition. eapply (H1 a); cset_tac; intuition.
-  - eauto.
-Qed.
-
-
-Lemma satisfiesAll_update_dead E Gamma Z vl
-: length Z = length vl
-  -> satisfiesAll E Gamma
-  -> eqns_freeVars Gamma ∩ of_list Z [=] ∅
-  -> satisfiesAll (E[Z <-- vl]) Gamma.
-Proof.
-  intros. hnf; intros.
-  exploit H0; eauto.
-  eapply satisfies_update_dead_list; eauto.
-  exploit eqns_freeVars_incl; eauto.
-  rewrite <- H1.
-  revert H1 X0; simpl; clear_all; cset_tac; intuition; exfalso; eauto.
-Qed.
-*)
-
 
 Lemma eval_op_subst E y Y Z e
 : length Z = length Y
@@ -186,156 +118,73 @@ Proof.
     erewrite IHe2; eauto.
 Qed.
 
-(*
-
-Lemma simL'_update r A (AR AR':ProofRelation A) LV L L' L1 L2
-: AIR5 (simB sim_progeq r AR) L L' LV L1 L2
-  -> (forall x b b', @BlockRel _ AR x b b' -> @BlockRel _ AR' x b b')
-  -> (forall a Z Z', @ParamRel _ AR a Z Z' -> @ParamRel _ AR' a Z Z')
-  -> (forall V V' a VL VL', @ArgRel _ AR V V' a VL VL' <-> @ArgRel _ AR' V V' a VL VL')
-  -> L = L1
-  -> L' = L2
-  -> AIR5 (simB sim_progeq r AR') L L' LV L1 L2.
+Lemma satisfies_subst V Z Y y bE gamma
+  (EVAL: omap (op_eval V) Y = ⎣ y ⎦)
+  (Len1 : ❬Y❭ = ❬y❭)
+  (Len2 : ❬Z❭ = ❬Y❭)
+  (AGR:agree_on eq (freeVars gamma \ of_list Z) V bE)
+  (SAT : satisfies V (subst_eqn (sid [Z <-- Y]) gamma))
+  : satisfies (bE [Z <-- Some ⊝ y]) gamma.
 Proof.
-  intros. revert_until H. remember AR. induction H; intros.
-  - econstructor.
-  - intros. invc H3. invc H4. inv pf.
-    econstructor; eauto.
-    econstructor; intros; eauto.
-    eapply H5; eauto. eapply H2; eauto.
+  hnf in SAT. destruct gamma; simpl in *.
+  * do 2 erewrite <- eval_op_subst in SAT; eauto.
+    erewrite op_eval_agree; [| |reflexivity].
+    erewrite op_eval_agree with (e:=e'); [| |reflexivity].
+    eapply SAT.
+    -- eapply update_with_list_agree; eauto with len.
+       eapply agree_on_incl; eauto. cset_tac.
+    -- eapply update_with_list_agree; eauto with len.
+       eapply agree_on_incl; eauto.
+       cset_tac.
+  * simpl in * |- *.
+    do 2 erewrite <- eval_op_subst in SAT; eauto.
+    erewrite op_eval_agree; [| |reflexivity].
+    erewrite op_eval_agree with (e:=e'); [| |reflexivity]; eauto.
+    -- eapply update_with_list_agree; eauto with len.
+       eapply agree_on_incl; eauto.
+       cset_tac.
+    -- eapply update_with_list_agree; eauto with len.
+       eapply agree_on_incl; eauto.
+       cset_tac.
+  * eauto.
 Qed.
-*)
-(*
-Lemma entails_freeVars_incl Gamma Γ' G x e
-: entails ({{(Var x, e)}} ∪ Gamma) Γ'
-  -> Exp.freeVars e ⊆ G
-  -> eqns_freeVars Gamma ⊆ G
-  -> eqns_freeVars Γ' ⊆ G ∪ {{x}}.
-Proof.
-  intros. destruct H.
-  rewrite eqns_freeVars_add in H2.
-  rewrite H2. unfold freeVars; simpl. rewrite H0. rewrite H1.
-  clear_all; cset_tac; intuition.
-Qed.
-*)
 
-
-
-Lemma satisfiesAll_subst V Gamma Z EqS Y y bE G
+Lemma satisfiesAll_subst V Gamma Z EqS Y y bE
 :  length Z = length Y
-   -> eqns_freeVars EqS ⊆ G ∪ of_list Z
    -> entails Gamma (subst_eqns (sid [Z <-- Y]) EqS)
    -> satisfiesAll V Gamma
-   -> agree_on eq G V bE
+   -> agree_on eq (eqns_freeVars EqS \ of_list Z) V bE
    -> omap (op_eval V) Y = ⎣y⎦
    -> satisfiesAll (bE [Z <-- List.map Some y]) EqS.
 Proof.
   revert_except EqS. pattern EqS. eapply set_induction; intros.
   - hnf; intros. eapply empty_is_empty_1 in H.
-    exfalso. rewrite H in H6. cset_tac; intuition.
+    exfalso. cset_tac.
   - hnf; intros.
     assert (LEN:❬Y❭ = ❬y❭). {
       eapply omap_length; eauto.
     }
-    eapply Add_Equal in H1. rewrite H1 in H8.
-    eapply add_iff in H8. destruct H8.
-    + hnf in H8; subst.
-      specialize (H4 V H5 (subst_eqn (sid [Z <-- Y]) gamma)).
-      exploit H4 as SAT.
-      eapply in_subst_eqns; eauto. rewrite H1. cset_tac.
-      hnf in SAT. destruct gamma. simpl in *.
-      * do 2 erewrite <- eval_op_subst in SAT; eauto.
-        erewrite op_eval_agree; [| |reflexivity].
-        erewrite op_eval_agree with (e:=e'); [| |reflexivity].
-        eapply SAT.
-        -- eapply update_with_list_agree; eauto with len.
-           eapply agree_on_incl; eauto.
-           assert (EqnEq e e' ∈ s') as IN. {
-             rewrite H1. cset_tac.
-           }
-           exploit eqns_freeVars_incl as FVI; eauto. simpl in *.
-           rewrite H3 in FVI. revert FVI; clear; cset_tac.
-        -- eapply update_with_list_agree; eauto with len.
-           eapply agree_on_incl; eauto.
-           assert (EqnEq e e' ∈ s') as IN. {
-             rewrite H1. cset_tac.
-           }
-           exploit eqns_freeVars_incl as FVI; eauto.
-           rewrite H3 in FVI. simpl in *.
-           revert FVI; clear; cset_tac.
-      * simpl in * |- *.
-        do 2 erewrite <- eval_op_subst in SAT; eauto.
-        erewrite op_eval_agree; [| |reflexivity].
-        erewrite op_eval_agree with (e:=e'); [| |reflexivity]; eauto.
-        -- eapply update_with_list_agree; eauto with len.
-           eapply agree_on_incl; eauto.
-           assert (EqnApx e e' ∈ s') as IN. {
-             rewrite H1. clear; cset_tac.
-           }
-           exploit eqns_freeVars_incl as FVI; eauto. simpl in *.
-           rewrite H3 in FVI.
-           revert FVI; clear; cset_tac.
-        -- eapply update_with_list_agree; eauto with len.
-           eapply agree_on_incl; eauto.
-           assert (EqnApx e e' ∈ s') as IN. {
-             rewrite H1. cset_tac.
-           }
-           exploit eqns_freeVars_incl as FVI; eauto.
-           rewrite H3 in FVI. simpl in *.
-           revert FVI; clear; cset_tac.
-      * simpl in *; eauto.
-    + rewrite H1 in H4.
-      eapply H; try eapply H7; eauto.
-      * rewrite <- H3. rewrite H1.
-        rewrite eqns_freeVars_add'. cset_tac; intuition.
-      * setoid_rewrite <- incl_add' in H4; eauto.
+    eapply Add_Equal in H1. rewrite H1 in *.
+    eapply add_iff in H7. destruct H7.
+    + hnf in H7; subst.
+      specialize (H3 V H4 (subst_eqn (sid [Z <-- Y]) gamma)).
+      exploit H3 as SAT.
+      * eapply in_subst_eqns; eauto. cset_tac.
+      * eapply satisfies_subst; eauto.
+        eapply agree_on_incl; eauto.
+        rewrite eqns_freeVars_add.
+        clear; cset_tac.
+    + eapply H; try eapply H7; eauto.
+      * etransitivity; eauto.
+        setoid_rewrite <- incl_add'; eauto. reflexivity.
+      * setoid_rewrite <- incl_add' in H5; eauto.
 Qed.
 
-
-(*
-Lemma satisfiesAll_update x Gamma V e e' y
-: x ∉ eqns_freeVars Gamma
-  -> x ∉ Exp.freeVars e
-  -> x ∉ Exp.freeVars e'
-  -> satisfiesAll V Gamma
-  -> ⎣y ⎦ = op_eval V e
-  -> ⎣y ⎦ = op_eval V e'
-  -> satisfiesAll (V [x <- ⎣y ⎦])
-                 ({EqnEq (Var x) e ; {EqnEq (Var x) e'; Gamma } }).
-Proof.
-  intros. hnf; intros. cset_tac. destruct H5 as [|[|]].
-  - invc H5; simpl in * |- *; subst.
-    + erewrite <- exp_eval_agree; eauto. instantiate (1:=V).
-      rewrite <- H3. simpl. lud. econstructor; eauto.
-      exfalso; eauto.
-      eapply agree_on_update_dead; eauto.
-  - invc H5; simpl in * |- *; subst.
-    + erewrite <- exp_eval_agree; eauto. instantiate (1:=V).
-      rewrite <- H4. simpl. lud. econstructor; eauto.
-      exfalso; eauto.
-      eapply agree_on_update_dead; eauto.
-  - hnf in H1. exploit H2; eauto.
-    eapply satisfies_update_dead; eauto.
-    intro. eapply in_eqns_freeVars in H6; eauto.
-Qed.
-
-
-Lemma satisfiesAll_update_dead_single x Gamma V y
-: x ∉ eqns_freeVars Gamma
-  -> satisfiesAll V Gamma
-  -> satisfiesAll (V [x <- ⎣y ⎦]) Gamma.
-Proof.
-  intros. hnf; intros.
-  - eapply satisfies_update_dead; eauto.
-    intro. eapply in_eqns_freeVars in H2; eauto.
-Qed.
-*)
-
-Lemma eqn_sound_monotone ZL Δ Γ Γ1 Γ1' s s' ang
+Lemma eqn_sound_monotone ZL Δ Γ Γ' s s' ang
   : renamedApart s ang
-    -> eqn_sound ZL Δ Γ s s' Γ1 ang
-    -> Γ1 ⊆ Γ1'
-    -> eqn_sound ZL Δ Γ s s' Γ1' ang.
+    -> eqn_sound ZL Δ s s' Γ ang
+    -> Γ ⊆ Γ'
+    -> eqn_sound ZL Δ s s' Γ' ang.
 Proof.
   intros. general induction H0;
             (try now (eapply EqnUnsat; eauto using unsatisfiable_monotone)); invt renamedApart; eauto.
@@ -366,11 +215,11 @@ Proof.
   intros. rewrite H. reflexivity.
 Qed.
 
-Lemma eqn_sound_entails_monotone ZL Δ Γ Γ1 Γ1' s s' ang
+Lemma eqn_sound_entails_monotone ZL Δ Γ1 Γ1' s s' ang
   : renamedApart s ang
-    -> eqn_sound ZL Δ Γ s s' Γ1 ang
+    -> eqn_sound ZL Δ s s' Γ1 ang
     -> entails Γ1' Γ1
-    -> eqn_sound ZL Δ Γ s s' Γ1' ang.
+    -> eqn_sound ZL Δ s s' Γ1' ang.
 Proof.
   intros. general induction H0;
             (try now (eapply EqnUnsat; eauto using unsatisfiable_entails_monotone));
@@ -404,80 +253,7 @@ Proof.
       eapply entails_incl. eauto with cset.
 Qed.
 
-
-(*
-Definition ArgRel' (Z:params ) (VL VL': list val) : Prop :=
-
-(*  /\ satisfiesAll ([Z <-- List.map Some VL]) (EqS ∪ Gamma)*).
-
-Definition ParamRel' (Zb:params) (Z Z' : list var) : Prop :=
- *)
-
-
-(*
-Lemma satisfies_omap_op_eval_some Gamma Y Y' V vl
-  : entails Gamma (list_EqnApx Y Y')
-    -> ❬Y❭ = ❬Y'❭
-    -> satisfiesAll V Gamma
-    -> omap (op_eval V) Y = ⎣ vl ⎦
-    -> omap (op_eval V) Y' = ⎣ vl ⎦.
-Proof.
-  intros.
-  exploit H; eauto.
-  case_eq (omap (op_eval V) Y); eauto.
-  intros. length_equify. general induction H0; simpl in * |- *; eauto using fstNoneOrR.
-  monad_inv H2. monad_inv H4. rewrite EQ0, EQ3. simpl. erewrite IHlength_eq; eauto.
-  - replace (op_eval V y) with ⎣x2⎦; simpl; eauto.
- *)
-
-
-
-
-
-
-(*
-  omap_satisfies_list_EqnApx, omap_exp_eval_onvLe
-*)
-
-
-
 Hint Resolve satisfies_fstNoneOrR_apx onvLe_fstNoneOrR_apx.
-
-Require Import MapDefined.
-
-(*
-we don't want to use this, because then we can't have if in the expression
-language anymore
-Lemma op_eval_fv_defined V e v
-  : op_eval V e = Some v
-    -> defined_on (Op.freeVars e) V.
-Proof.
-  unfold defined_on.
-  general induction e; simpl in *; cset_tac'.
-  - monad_inv H. cset_tac'.
-  - monad_inv H. cset_tac'.
-  - monad_inv H. cset_tac'.
-Qed.
-
-Lemma test Gamma e e'
-  : entails Gamma {EqnApx e e'}
-    -> (exists V v, satisfiesAll V Gamma /\ op_eval V e = Some v)
-    -> Op.freeVars e' ⊆ Op.freeVars e ∪ eqns_freeVars Gamma.
-Proof.
-  intros. decide (Op.freeVars e' ⊆ Op.freeVars e ∪ eqns_freeVars Gamma); eauto.
-  eapply not_incl_exists in n. dcr. exfalso.
-  assert (satisfiesAll (fun y => if [y === x] then None else x0 y) Gamma). {
-    eapply satisfiesAll_agree; eauto.
-    hnf; intros. cases; eauto. cset_tac.
-  }
-  eapply H in H0.
-  eapply satisfies_single' in H0. simpl in *.
-  erewrite op_eval_agree in H0; eauto.
-  inv H0. exploit op_eval_fv_defined. symmetry. eauto.
-  exploit H4; eauto. dcr. cases in H8; isabsurd.
-  hnf; intros. cases; eauto. cset_tac.
-Qed.
-*)
 
 Instance PR : PointwiseProofRelationF (params*eqns):=
   {
@@ -490,17 +266,16 @@ Instance PR : PointwiseProofRelationF (params*eqns):=
     ParamRelFP := fun '(Z,_) Z' Zb => Z = Z' /\ Zb = Z'
   }.
 
-Lemma sim_vopt r L L' V V' s s' ZL Δ ΓL Gamma ang
+Lemma sim_vopt r L L' V V' s s' ZL Δ Gamma ang
   : satisfiesAll V Gamma
-    -> eqn_sound ZL Δ ΓL s s' Gamma ang
-    -> labenv_sim Sim (sim r) PR (zip pair ZL ΓL) L L'
+    -> eqn_sound ZL Δ s s' Gamma ang
+    -> labenv_sim Sim (sim r) PR (zip pair ZL Δ) L L'
     -> renamedApart s ang
     -> eqns_freeVars Gamma ⊆ fst (getAnn ang)
     -> onvLe V V'
-    -> (forall n b G Γf, get L n b ->
-                get Δ n G ->
-                get ΓL n Γf ->
-                G ⊆ fst (getAnn ang) /\
+    -> (forall n b Γf, get L n b ->
+                get Δ n Γf ->
+                exists G, G ⊆ fst (getAnn ang) /\
                 eqns_freeVars Γf ⊆ G ∪ of_list (block_Z b) /\
                 agree_on eq G (F.block_E b) V)
     -> sim r Sim  (L,V, s) (L',V', s').
@@ -524,7 +299,7 @@ Proof.
         rewrite H7, FV. clear. cset_tac.
       * eapply agree_on_onvLe; eauto.
       * intros. exploit EEQ; dcr; eauto.
-        pe_rewrite. do 2 try split; eauto with cset.
+        pe_rewrite. exists x0. do 2 try split; eauto with cset.
         symmetry. eapply agree_on_update_dead; eauto.
         symmetry; eauto.
   -  exploit H; eauto.  exploit H0; eauto; [cset_tac|].
@@ -549,7 +324,7 @@ Proof.
     exploit EEQ; eauto; dcr. simpl in *.
     repeat split; eauto.
     + symmetry; eapply agree_on_incl; eauto.
-      rewrite H14; eauto. clear; cset_tac.
+      rewrite H11; eauto. clear; cset_tac.
   - eapply (sim_return_apx il_statetype_F).
     exploit H; eauto. exploit H0; eauto; [cset_tac|]. etransitivity; eauto.
   - exploit H; eauto. eapply (sim_let_call_apx il_statetype_F); eauto; simpl.
@@ -562,7 +337,7 @@ Proof.
         rewrite FV.  clear_all. cset_tac.
       * eauto using agree_on_onvLe.
       * intros. exploit EEQ; dcr; eauto.
-        pe_rewrite. do 2 try split; eauto with cset.
+        pe_rewrite. eexists x0. do 2 try split; eauto with cset.
         symmetry. eapply agree_on_update_dead; eauto.
         symmetry; eauto.
   - pone_step. left. eapply IHEQN; eauto.
@@ -574,8 +349,7 @@ Proof.
         -- rewrite satisfiesAll_union; split.
            ++ exploit EqnFVF; eauto.
              edestruct H8; eauto; dcr. simpl in *.
-             eapply satisfiesAll_subst
-             with (G:=eqns_freeVars x0 \ of_list Z); eauto.
+             eapply satisfiesAll_subst; eauto.
              eauto with len.
              eauto with cset.
              eapply satisfiesAll_union; split; eauto.
@@ -596,34 +370,30 @@ Proof.
            clear; cset_tac.
         -- exploit ParamEq; dcr; eauto; subst.
            eapply agree_on_onvLe_update_list. eauto.
-        -- intros. eapply get_app_cases in H16. destruct H16.
-           ++ inv_get. edestruct H8; try eapply H13; eauto; dcr. simpl in *.
-             rewrite H15. split; eauto with cset.
-             exploit EqnFVF; eauto.
-             rewrite get_app_lt in H14; eauto with len. inv_get. simpl in *.
-             rewrite H5; split; eauto.
+        -- intros ? ? ? Get1 Get2. eapply get_app_cases in Get1. destruct Get1.
+           ++ inv_get.
+             edestruct H8; try eapply H13; eauto; dcr. simpl in *.
+             eexists G. rewrite H15. split; eauto with cset.
+             exploit EqnFVF; eauto. split; eauto.
              eapply agree_on_update_list_dead; eauto with len.
-           ++ dcr; simpl in *. rewrite Len1 in *.
-             rewrite get_app_ge in H14; eauto with len.
-             rewrite get_app_ge in H15; eauto with len.
-             len_simpl.
+           ++ dcr; simpl in *. len_simpl.
+             rewrite get_app_ge in Get2; eauto with len.
+             rewrite Len1 in *. inv_get.
              exploit EEQ; eauto; dcr.
              edestruct H8; try eapply H13; eauto; dcr.
+             eexists x4.
              rewrite H5. simpl. split. eauto with cset.
              simpl in *. split; eauto.
              eapply agree_on_update_list_dead; eauto.
-             rewrite H23. eauto.
+             rewrite H21. eauto. omega.
       * hnf. intros. simpl in *. subst. inv_get. exploit ParamEq; dcr; eauto.
     + pe_rewrite. eauto.
-    + intros. eapply get_app_cases in H2. destruct H2.
-      ++ inv_get. pe_rewrite. split; eauto.
-        exploit EqnFVF; eauto.
-        rewrite get_app_lt in H0; eauto with len. inv_get. simpl in *.
-        rewrite H1; split; eauto.
-      ++ dcr; simpl in *. rewrite Len1 in *.
-        rewrite get_app_ge in H0; eauto with len.
-        rewrite get_app_ge in H1; eauto with len.
-        len_simpl.
+    + intros ? ? ? Get1 Get2. eapply get_app_cases in Get1. destruct Get1.
+      ++ inv_get. pe_rewrite. eexists G; split; eauto.
+      ++ dcr; simpl in *. len_simpl.
+        rewrite get_app_ge in Get2; eauto with len.
+        rewrite Len1 in *.
         exploit EEQ; eauto; dcr.
-        pe_rewrite. split; eauto.
+        eexists x. split; eauto. pe_rewrite. eauto.
+        omega.
 Qed.
